src/Slabs: remove allocate_slot_refined admit
more precisely, move it to Utils2
falls under the group of
sizeclass bitwise ops issues,
that is, progress has to be made on
size classes range for this to be fixed

src/Slots.fst
@@ -521,7 +521,7 @@ let get_free_slot (size_class: sc) (bitmap: slab_metadata)
     get_free_slot_aux size_class bitmap 0ul
   )
 
-#push-options "--z3rlimit 30"
+#push-options "--z3rlimit 50"
 let allocate_slot
   (size_class: sc)
   (md: slab_metadata)
@@ -541,7 +541,9 @@ let allocate_slot
       = h1 (slab_vprop size_class arr md) in
     let v0 : Seq.lseq U64.t 4 = dfst blob0 in
     let v1 : Seq.lseq U64.t 4 = dfst blob1 in
-    True)
+    not (is_empty size_class v1))
+    //U32.v (G.reveal (snd r)) < U64.n * 4 /\
+    //v1 == Bitmap4.set v0 (G.reveal (snd r)))
     //TODO: is it worth having such a precise spec?
     //requires having pos as ghost in returned value
     //considering the case of multiple consecutive allocations
@@ -565,6 +567,8 @@ let allocate_slot
     md_as_seq2
     arr
     pos in
+  let md_as_seq3 = gget (A.varray md) in
+  set_lemma_nonzero size_class (G.reveal md_as_seq2) (G.reveal md_as_seq3) pos;
   intro_vdep
     (A.varray md)
     (slab_vprop_aux size_class arr (Bitmap4.set md_as_seq2 pos))
